rework shared prefixes, refactor SQ.thy
fix important shared prefix lemmas that were using dlog where they should be using clog (a notable change is the new minimum word length of 20)
create supplementary theory sublists for `suffix` related lemmas

rework shared prefix definitions:
- rename to `shared_MSBs` (most significant bits) to avoid confusion around prefix/suffix
- change from existance based defs (see for instance `suffix`) to functional definitions
- many basic lemmas (such as a shared prefix of length n implying a shared prefix of length m <= n) are trivial with the new definitions
- the definitions fit better into the next level of theorems

papers/116_stefan_rass/L0.thy
@@ -106,52 +106,36 @@ definition L\<^sub>0' :: lang
   where L0'_def[simp]: "L\<^sub>0' \<equiv> L\<^sub>D' \<inter> SQ"
 
 
-definition adj_sq\<^sub>w :: "word \<Rightarrow> word"
-  where adj_sq_word_def[simp]: "adj_sq\<^sub>w w \<equiv> gn_inv (adj_square (gn w))"
-
-
-lemma adj_sq_word_correct: "adj_sq\<^sub>w w \<in> SQ" unfolding adj_sq_word_def SQ_def
-  using adj_sq_correct and adj_sq_gt_0 by (intro CollectI) (subst inv_gn_id)
-
-lemma adj_sq_word_length: 
-  fixes w
-  assumes "length w \<ge> 7"
-    \<comment> \<open>Otherwise, \<^term>\<open>2 ^ suffix_len (gn w) > bit_length (gn w)\<close>,
-        and \<^term>\<open>(gn w) - (gn w) mod 2^(suffix_len (gn w)) = 0\<close>.\<close>
-  shows "length (adj_sq\<^sub>w w) = length w" sorry
-\<comment> \<open>Proof idea: one bit is added in \<^const>\<open>gn\<close>, one removed in \<^const>\<open>gn_inv\<close>.
-    As \<^const>\<open>gn\<close> appends a \<open>1\<close>, possible leading zeroes are avoided.\<close>
-
-
 lemma adj_sq_exp_pad:
   fixes w
-  assumes "length w \<ge> 18"
-  defines "w' \<equiv> adj_sq\<^sub>w w"
+  defines l: "l \<equiv> length w"
+    and w': "w' \<equiv> adj_sq\<^sub>w w"
+  assumes "l \<ge> 20"
   shows "strip_exp_pad w' = strip_exp_pad w"
 proof -
-  define l where "l \<equiv> length w"
-  have len_eq: "length w' = l" unfolding l_def w'_def using \<open>length w \<ge> 18\<close>
-    by (intro adj_sq_word_length) linarith
+  from \<open>l \<ge> 20\<close> have "shared_MSBs (clog l) w w'" unfolding l w' by (rule adj_sq_sh_pfx_log)
+  then have l_eq: "length w' = l" and d_eq: "drop (l - clog l) w' = drop (l - clog l) w"
+    unfolding l by (elim sh_msbE[symmetric])+
 
-  have "strip_exp_pad w' = drop (l - clog l) w'" unfolding strip_exp_pad_def len_eq Let_def ..
-  also have "... = drop (l - clog l) w" sorry (* shared prefix *)
-  also have "... = strip_exp_pad w" unfolding strip_exp_pad_def l_def[symmetric] Let_def ..
+  have "strip_exp_pad w' = drop (l - clog l) w'" unfolding strip_exp_pad_def l_eq Let_def ..
+  also have "... = drop (l - clog l) w" using d_eq .
+  also have "... = strip_exp_pad w" unfolding strip_exp_pad_def l[symmetric] Let_def ..
   finally show ?thesis .
 qed
 
 corollary adj_sq_TM_dec:
   fixes w
-  assumes "length w \<ge> 18"
+  assumes "length w \<ge> 20"
   defines "w' \<equiv> adj_sq\<^sub>w w"
   shows "TM_decode_pad w' = TM_decode_pad w"
-  unfolding TM_decode_pad_def w'_def using \<open>length w \<ge> 18\<close> by (subst adj_sq_exp_pad) fast+
+  unfolding TM_decode_pad_def w'_def using \<open>length w \<ge> 20\<close> by (subst adj_sq_exp_pad) fast+
 
 lemma L\<^sub>D_adj_sq_iff:
   fixes w
-  assumes "length w \<ge> 18"
+  assumes "length w \<ge> 20"
   defines "w' \<equiv> adj_sq\<^sub>w w"
   shows "w' \<in> L\<^sub>D \<longleftrightarrow> w \<in> L\<^sub>D"
-    \<comment> \<open>Idea: since \<open>n\<close> and \<open>adj_square n\<close> share their prefix (@{thm adj_sq_shared_prefix_log}),
+    \<comment> \<open>Idea: since \<open>w\<close> and \<open>adj_sq\<^sub>w n\<close> share their prefix (@{thm adj_sq_sh_pfx_log}),
   the relevant parts are identical and this lemma should hold.
 
   Note: with the current definition of \<^const>\<open>L\<^sub>D\<close>, this likely does not hold,
@@ -161,19 +145,20 @@ lemma L\<^sub>D_adj_sq_iff:
 
 lemma L\<^sub>D'_adj_sq_iff:
   fixes w
-  assumes l: "length w \<ge> 18"
+  assumes l: "length w \<ge> 20"
   defines w': "w' \<equiv> adj_sq\<^sub>w w"
   shows "w' \<in> L\<^sub>D' \<longleftrightarrow> w \<in> L\<^sub>D'"
 proof -
+  from \<open>length w \<ge> 20\<close> have "shared_MSBs (clog (length w)) w w'" unfolding w' by (rule adj_sq_sh_pfx_log)
+  then have len: "length w' = length w" by (elim sh_msbE[symmetric])
   from l have dec: "TM_decode_pad w' = TM_decode_pad w" unfolding w' by (rule adj_sq_TM_dec)
   from l have pad: "strip_exp_pad w' = strip_exp_pad w" unfolding w' by (rule adj_sq_exp_pad)
-  from l have len: "length w' = length w" unfolding w' by (intro adj_sq_word_length) force
   show "w' \<in> L\<^sub>D' \<longleftrightarrow> w \<in> L\<^sub>D'" unfolding LD'_def mem_Collect_eq unfolding dec pad len ..
 qed
 
 lemma L\<^sub>D'_L\<^sub>0'_adj_sq_iff:
   fixes w
-  assumes l: "length w \<ge> 18"
+  assumes l: "length w \<ge> 20"
   defines "w' \<equiv> adj_sq\<^sub>w w"
   shows "w \<in> L\<^sub>D' \<longleftrightarrow> w' \<in> L\<^sub>0'"
 proof
